LocalLang/SemanticsLemmas.lean
@@ -1,0 +1,18 @@
+import LocalLang.Semantics
+
+instance {defs : Definitions} :
+  Trans (SmallStep defs V) (SmallStep defs V) (SmallSteps defs V) where
+    trans st₁ st₂ := Relation.ReflTransGen.trans
+      (Relation.ReflTransGen.single st₁) (Relation.ReflTransGen.single st₂)
+
+lemma head_step_implies_context_step {e₁ e₂ e₁' e₂' : Expr} {V V' : Env} {defs : Definitions}
+  (st : HeadSmallStep defs V' e₁ e₂) (ctx : Ctx) (HEnv : V' = ctx.updateEnv V)
+  (He₁ : e₁' = ctx.fill e₁) (He₂ : e₂' = ctx.fill e₂) : SmallStep defs V e₁' e₂' := by
+  rw [HEnv] at st
+  let result := SmallStep.ctx_step ctx V st
+  rw [← He₁, ← He₂] at result
+  assumption
+
+lemma steps_in_context_imply_steps_in_expr {e₁ e₂ e₁' e₂' : Expr} {V V' : Env} {defs : Definitions}
+  (sts : SmallSteps defs V' e₁ e₂) (ctx : Ctx) (HEnv : V' = ctx.updateEnv V)
+  (He₁ : e₁' = ctx.fill e₁) (He₂ : e₂' = ctx.fill e₂) : SmallSteps defs V e₁' e₂' := by sorry
